example/out/ProcDecExec.v
@@ -2,6 +2,7 @@ Require Import Bool String List Arith.
 Require Import Omega.
 Require Import Kami.All.
 Require Import Bsvtokami.
+Require Import Decoder.
 
 Require Import FunctionalExtensionality.
 
@@ -12,129 +13,134 @@ Require Import FIFO.
 Require Import RegFile.
 Require Import ProcMemSpec.
 Require Import PipelinedProc.
+Require Import Vector.
 Module module'mkDecExec.
     Section Section'mkDecExec.
     Variable instancePrefix: string.
-    Variable pgm: RegFile.
-    Variable dec: Decoder.
-    Variable exec: Executer.
-    Variable sb: Scoreboard.
-    Variable e2wFifo: FIFO.
-    Variable rf: ProcRegs.
-    Variable mem: Memory.
-    Variable toHost: ToHost.
+    Variable pgm: string.
+    Variable dec: Decoder.Decoder.
+    Variable exec: Decoder.Executer.
+    Variable e2wFifo_reg: string.
+    Variable e2wFifo_valid: string.
+    Variable rf: string.
+    Variable mem: string.
+    Variable toHost: string.
         (* method bindings *)
-    Let pc := mkReg (instancePrefix--"pc") (natToWord PgmSz 0)%bk.
-    Let pc_read : string := (Reg'_read pc).
-    Let pc_write : string := (Reg'_write pc).
+    Let pc : string := instancePrefix--"pc".
+    Let sbFlags : string := instancePrefix--"sbFlags".
     (* instance methods *)
-    Let decgetAddr : string := (Decoder'getAddr dec).
-    Let decgetArithOp : string := (Decoder'getArithOp dec).
-    Let decgetDst : string := (Decoder'getDst dec).
-    Let decgetSrc1 : string := (Decoder'getSrc1 dec).
-    Let decgetSrc2 : string := (Decoder'getSrc2 dec).
-    Let decisOp : string := (Decoder'isOp dec).
-    Let e2wFifoenq : string := (FIFO'enq e2wFifo).
-    Let execexecArith : string := (Executer'execArith exec).
-    Let memdoMem : string := (Memory'doMem mem).
-    Let pgmsub : string := (RegFile'sub pgm).
-    Let rfread1 : string := (ProcRegs'read1 rf).
-    Let rfread2 : string := (ProcRegs'read2 rf).
-    Let sbinsert : string := (Scoreboard'insert sb).
-    Let sbsearch1 : string := (Scoreboard'search1 sb).
-    Let sbsearch2 : string := (Scoreboard'search2 sb).
-    Let toHosttoHost : string := (ToHost'toHost toHost).
+    Let mem'doMem : string := mem--"doMem".
+    Let toHost'toHost : string := toHost--"toHost".
     Local Open Scope kami_expr.
 
     Definition mkDecExecModule: Mod :=
          (BKMODULE {
-        (BKMod (Reg'mod pc :: nil))
+        Register pc : Bit PgmSz <- natToWord PgmSz 0
+    with Register sbFlags : Array NumRegs Bool <- Default
     with Rule instancePrefix--"decexecArith" :=
     (
-        Call pc_v : Bit PgmSz (* regRead *) <- pc_read() ;
-       Call call12 : Bit InstrSz <-  pgmsub ((#pc_v) : Bit PgmSz) ;
-       BKCall call11 : Bool <-  decisOp ((#call12) : Bit InstrSz) (($$opArith) : OpK) ;
-       Call call15 : Bit InstrSz <-  pgmsub ((#pc_v) : Bit PgmSz) ;
-       Call call14 : Bit RegFileSz <-  decgetSrc1 ((#call15) : Bit InstrSz) ;
-       Call call13 : Bool <-  sbsearch1 ((#call14) : Bit RegFileSz) ;
-       Call call18 : Bit InstrSz <-  pgmsub ((#pc_v) : Bit PgmSz) ;
-       Call call17 : Bit RegFileSz <-  decgetSrc2 ((#call18) : Bit InstrSz) ;
-       Call call16 : Bool <-  sbsearch2 ((#call17) : Bit RegFileSz) ;
+        Read e2wFifo_valid_v : Bool <- e2wFifo_valid ;
+        Read pc_v : Bit PgmSz <- pc ;
+        Read sbFlags_v : Array NumRegs Bool <- sbFlags ;
+       Read instrs : Array NumInstrs (Bit InstrSz) <- pgm ;
+       LET call17 : Bit InstrSz <- #instrs @[  #pc_v ] ;
+       LET call16 : Bool <- (getOp dec _ call17) == $$opArith ;
+       LET call19 : Bit InstrSz <- #instrs @[ #pc_v ] ;
+       LET call18 : Bit RegFileSz <-  getSrc1 dec _ call19 ;
+       LET call21 : Bit InstrSz <-  #instrs @[ #pc_v ] ;
+       LET call20 : Bit RegFileSz <-  getSrc2 dec _ call21 ;
 
-        Assert(((#call11 && (!#call13)) && (!#call16))) ;
-       Call inst : Bit InstrSz (* varbinding *) <-  pgmsub ((#pc_v) : Bit PgmSz) ;
-       Call src1 : Bit RegFileSz (* varbinding *) <-  decgetSrc1 ((#inst) : Bit InstrSz) ;
-       Call src2 : Bit RegFileSz (* varbinding *) <-  decgetSrc2 ((#inst) : Bit InstrSz) ;
-       Call dst : Bit RegFileSz (* varbinding *) <-  decgetDst ((#inst) : Bit InstrSz) ;
-       Call arithOp : OpArithK (* varbinding *) <-  decgetArithOp ((#inst) : Bit InstrSz) ;
-       Call val1 : Bit DataSz (* varbinding *) <-  rfread1 ((#src1) : Bit RegFileSz) ;
-       Call val2 : Bit DataSz (* varbinding *) <-  rfread2 ((#src2) : Bit RegFileSz) ;
-       BKCall execVal : Bit DataSz (* varbinding *) <-  execexecArith ((#arithOp) : OpArithK) ((#val1) : Bit DataSz) ((#val2) : Bit DataSz) ;
-               Call inserted : Void (* actionBinding *) <- sbinsert ((#dst) : Bit RegFileSz) ;
-               LET e2w : E2W <- STRUCT { "idx" ::= (#dst) ; "val" ::= (#execVal)  }%kami_expr ;
-               Call enq : Void (* actionBinding *) <- e2wFifoenq ((#e2w) : E2W) ;
-               Call pc_write ( ((#pc_v + $1)) : Bit PgmSz ) ;
+        Assert((((#call16 && (!(#sbFlags_v @[ #call18 ]))) && (!(#sbFlags_v @[ #call20 ]))) && (!#e2wFifo_valid_v))) ;
+       LET inst : Bit InstrSz (* varbinding *) <-  #instrs @[ #pc_v ] ;
+       LET src1 : Bit RegFileSz (* varbinding *) <-  getSrc1 dec _ inst ;
+       LET src2 : Bit RegFileSz (* varbinding *) <-  getSrc2 dec _ inst ;
+       LET dst : Bit RegFileSz (* varbinding *) <-  getDst dec _ inst ;
+       LET arithOp : OpArithK (* varbinding *) <- getArithOp dec _ inst ;
+       Read regsval : Array NumRegs (Bit DataSz) <- rf ;
+       LET val1 : Bit DataSz (* varbinding *) <-  #regsval @[ #src1 ] ;
+       LET val2 : Bit DataSz (* varbinding *) <-  #regsval @[ #src2 ] ;
+       LET execVal : Bit DataSz <- (execArith exec _ arithOp val1 val2) ;
+               LET flags : Array NumRegs Bool (* non-call varbinding *) <- #sbFlags_v ;
+               LET flags : Array NumRegs Bool <- #flags @[#dst <- $$true] ;
+               Write sbFlags : Array NumRegs Bool <- #flags ;
+               LET e2w : E2W (* non-call varbinding *) <- STRUCT { "idx" ::= (#dst) ; "val" ::= (#execVal)  }%kami_expr ;
+               Write e2wFifo_reg : E2W <- #e2w ;
+               Write e2wFifo_valid : Bool <- ($$true)%kami_expr ;
+               Write pc : Bit PgmSz <- (#pc_v + $$ (* intwidth *) (natToWord PgmSz 1)) ;
         Retv ) (* rule decexecArith *)
     with Rule instancePrefix--"decexecLd" :=
     (
-        Call pc_v : Bit PgmSz (* regRead *) <- pc_read() ;
-       Call call20 : Bit InstrSz <-  pgmsub ((#pc_v) : Bit PgmSz) ;
-       BKCall call19 : Bool <-  decisOp ((#call20) : Bit InstrSz) (($$opLd) : OpK) ;
-       Call call23 : Bit InstrSz <-  pgmsub ((#pc_v) : Bit PgmSz) ;
-       Call call22 : Bit RegFileSz <-  decgetDst ((#call23) : Bit InstrSz) ;
-       Call call21 : Bool <-  sbsearch1 ((#call22) : Bit RegFileSz) ;
+        Read e2wFifo_valid_v : Bool <- e2wFifo_valid ;
+        Read pc_v : Bit PgmSz <- pc ;
+        Read sbFlags_v : Array NumRegs Bool <- sbFlags ;
+       Read instrs : Array NumInstrs (Bit InstrSz) <- pgm ;
+       LET call23 : Bit InstrSz <- #instrs @[ #pc_v ] ;
+       LET call22 : Bool <-  (getOp dec _ call23) == $$opLd ;
+       LET call25 : Bit InstrSz <-  #instrs @[ #pc_v ] ;
+       LET call24 : Bit RegFileSz <-  getDst dec _ call25 ;
 
-        Assert((#call19 && (!#call21))) ;
-       Call inst : Bit InstrSz (* varbinding *) <-  pgmsub ((#pc_v) : Bit PgmSz) ;
-       Call src1 : Bit RegFileSz (* varbinding *) <-  decgetSrc1 ((#inst) : Bit InstrSz) ;
-       Call dst : Bit RegFileSz (* varbinding *) <-  decgetDst ((#inst) : Bit InstrSz) ;
-       Call addr : Bit AddrSz (* varbinding *) <-  decgetAddr ((#inst) : Bit InstrSz) ;
-       Call val1 : Bit DataSz (* varbinding *) <-  rfread1 ((#src1) : Bit RegFileSz) ;
-               LET memrq : MemRq <- STRUCT { "addr" ::= (#addr) ; "data" ::= (#val1) ; "isLoad" ::= ($$ (natToWord 1 1))  }%kami_expr ;
-               Call ldVal : Bit DataSz (* actionBinding *) <- memdoMem ((#memrq) : MemRq) ;
-               Call inserted : Void (* actionBinding *) <- sbinsert ((#dst) : Bit RegFileSz) ;
-               LET e2w : E2W <- STRUCT { "idx" ::= (#dst) ; "val" ::= (#ldVal)  }%kami_expr ;
-               Call enq : Void (* actionBinding *) <- e2wFifoenq ((#e2w) : E2W) ;
-               Call pc_write ( ((#pc_v + $1)) : Bit PgmSz ) ;
+        Assert(((#call22 && (!(#sbFlags_v @[ #call24 ]))) && (!#e2wFifo_valid_v))) ;
+       LET inst : Bit InstrSz (* varbinding *) <- #instrs @[ #pc_v ] ;
+       LET src1 : Bit RegFileSz (* varbinding *) <-  getSrc1 dec _ inst ;
+       LET dst : Bit RegFileSz (* varbinding *) <-  getDst dec _ inst ;
+       LET addr : Bit AddrSz (* varbinding *) <- getAddr dec _ inst ;
+       Read regsval : Array NumRegs (Bit DataSz) <- rf ;
+       LET val1 : Bit DataSz (* varbinding *) <-  #regsval @[ #src1 ] ;
+
+               LET memrq : MemRq (* non-call varbinding *) <- STRUCT { "addr" ::= (#addr) ; "data" ::= (#val1) ; "isLoad" ::= ($$ (* intwidth *) (natToWord 1 1))  }%kami_expr ;
+               BKCall ldVal : Bit DataSz (* actionBinding *) <- mem'doMem ((#memrq) : MemRq) ;
+               LET flags : Array NumRegs Bool (* non-call varbinding *) <- #sbFlags_v ;
+               LET flags : Array NumRegs Bool <- #flags @[#dst <- $$true ] ;
+               Write sbFlags : Array NumRegs Bool <- #flags ;
+               LET e2w : E2W (* non-call varbinding *) <- STRUCT { "idx" ::= (#dst) ; "val" ::= (#ldVal)  }%kami_expr ;
+               Write e2wFifo_reg : E2W <- #e2w ;
+               Write e2wFifo_valid : Bool <- ($$true)%kami_expr ;
+               Write pc : Bit PgmSz <- (#pc_v + $$ (* intwidth *) (natToWord PgmSz 1)) ;
         Retv ) (* rule decexecLd *)
     with Rule instancePrefix--"decexecSt" :=
     (
-        Call pc_v : Bit PgmSz (* regRead *) <- pc_read() ;
-       Call call25 : Bit InstrSz <-  pgmsub ((#pc_v) : Bit PgmSz) ;
-       BKCall call24 : Bool <-  decisOp ((#call25) : Bit InstrSz) (($$opSt) : OpK) ;
+        Read pc_v : Bit PgmSz <- pc ;
+       Read instrs : Array NumInstrs (Bit InstrSz) <- pgm ;
+       LET call27 : Bit InstrSz <-  #instrs @[ #pc_v ] ;
+       LET call26 : Bool <-  (getOp dec _ call27)  == $$opSt ;
 
-        Assert(#call24) ;
-       Call inst : Bit InstrSz (* varbinding *) <-  pgmsub ((#pc_v) : Bit PgmSz) ;
-       Call src1 : Bit RegFileSz (* varbinding *) <-  decgetSrc1 ((#inst) : Bit InstrSz) ;
-       Call addr : Bit AddrSz (* varbinding *) <-  decgetAddr ((#inst) : Bit InstrSz) ;
-       Call val1 : Bit DataSz (* varbinding *) <-  rfread1 ((#src1) : Bit RegFileSz) ;
-               LET memrq : MemRq <- STRUCT { "addr" ::= (#addr) ; "data" ::= (#val1) ; "isLoad" ::= ($$ (natToWord 1 0))  }%kami_expr ;
-               Call unused : Bit DataSz (* actionBinding *) <- memdoMem ((#memrq) : MemRq) ;
-               Call pc_write ( ((#pc_v + $1)) : Bit PgmSz ) ;
+        Assert(#call26) ;
+       LET inst : Bit InstrSz (* varbinding *) <- #instrs @[ #pc_v ] ;
+       LET src1 : Bit RegFileSz (* varbinding *) <- getSrc1 dec _ inst ;
+       LET addr : Bit AddrSz (* varbinding *) <-  getAddr dec _ inst ;
+       Read regsval : Array NumRegs (Bit DataSz) <- rf ;
+       LET val1 : Bit DataSz (* varbinding *) <-  #regsval @[ #src1 ] ;
+               LET memrq : MemRq (* non-call varbinding *) <- STRUCT { "addr" ::= (#addr) ; "data" ::= (#val1) ; "isLoad" ::= ($$ (* intwidth *) (natToWord 1 0))  }%kami_expr ;
+               BKCall unused : Bit DataSz (* actionBinding *) <- mem'doMem ((#memrq) : MemRq) ;
+               Write pc : Bit PgmSz <- (#pc_v + $$ (* intwidth *) (natToWord PgmSz 1)) ;
         Retv ) (* rule decexecSt *)
     with Rule instancePrefix--"decexecToHost" :=
     (
-        Call pc_v : Bit PgmSz (* regRead *) <- pc_read() ;
-       Call call27 : Bit InstrSz <-  pgmsub ((#pc_v) : Bit PgmSz) ;
-       BKCall call26 : Bool <-  decisOp ((#call27) : Bit InstrSz) (($$opTh) : OpK) ;
-       Call call30 : Bit InstrSz <-  pgmsub ((#pc_v) : Bit PgmSz) ;
-       Call call29 : Bit RegFileSz <-  decgetSrc1 ((#call30) : Bit InstrSz) ;
-       Call call28 : Bool <-  sbsearch1 ((#call29) : Bit RegFileSz) ;
+        Read pc_v : Bit PgmSz <- pc ;
+        Read sbFlags_v : Array NumRegs Bool <- sbFlags ;
+       Read instrs : Array NumInstrs (Bit InstrSz) <- pgm ;
+       LET call29 : Bit InstrSz <-  #instrs @[  #pc_v ] ;
+       LET call28 : Bool <-  (getOp dec _ call29) == $$opTh ;
+       LET call31 : Bit InstrSz <-  #instrs @[ #pc_v ] ;
+       LET call30 : Bit RegFileSz <-  getSrc1 dec _ call31 ;
 
-        Assert((#call26 && (!#call28))) ;
-       Call inst : Bit InstrSz (* varbinding *) <-  pgmsub ((#pc_v) : Bit PgmSz) ;
-       Call src1 : Bit RegFileSz (* varbinding *) <-  decgetSrc1 ((#inst) : Bit InstrSz) ;
-       Call val1 : Bit DataSz (* varbinding *) <-  rfread1 ((#src1) : Bit RegFileSz) ;
-               Call unused : Void (* actionBinding *) <- toHosttoHost ((#val1) : Bit DataSz) ;
-               Call pc_write ( ((#pc_v + $1)) : Bit PgmSz ) ;
+        Assert((#call28 && (!(#sbFlags_v @[ #call30 ])))) ;
+       LET inst : Bit InstrSz (* varbinding *) <-  #instrs @[ #pc_v ] ;
+       LET src1 : Bit RegFileSz (* varbinding *) <- getSrc1 dec _ inst ;
+       Read regsval : Array NumRegs (Bit DataSz) <- rf ;
+       LET val1 : Bit DataSz (* varbinding *) <-  #regsval @[ #src1 ] ;
+
+               BKCall unused : Void (* actionBinding *) <- toHost'toHost ((#val1) : Bit DataSz) ;
+               Write pc : Bit PgmSz <- (#pc_v + $$ (* intwidth *) (natToWord PgmSz 1)) ;
         Retv ) (* rule decexecToHost *)
     }). (* mkDecExec *)
 
     Hint Unfold mkDecExecModule : ModuleDefs.
-
-(* Module mkDecExec type RegFile#(Bit#(PgmSz), Bit#(InstrSz)) -> Decoder -> Executer -> Scoreboard -> FIFO#(E2W) -> ProcRegs -> Memory -> ToHost -> Module#(Empty) return type Decoder *)
-    Definition mkDecExec := Build_Empty mkDecExecModule%kami.
+(* Module mkDecExec type RegFile#(Bit#(PgmSz), Bit#(InstrSz)) -> Decoder -> Executer -> Reg#(E2W) -> Reg#(Bool) -> ProcRegs -> Memory -> ToHost -> Module#(Empty) return type Decoder *)
+    Definition mkDecExec := Build_Empty mkDecExecModule.
     Hint Unfold mkDecExec : ModuleDefs.
+    Hint Unfold mkDecExecModule : ModuleDefs.
+
     End Section'mkDecExec.
 End module'mkDecExec.
 
@@ -146,33 +152,145 @@ Hint Unfold module'mkDecExec.mkDecExecModule : ModuleDefs.
 Module module'mkDecExecSep.
     Section Section'mkDecExecSep.
     Variable instancePrefix: string.
-    Variable pgm: RegFile.
-    Variable dec: Decoder.
-    Variable exec: Executer.
-    Variable toHost: ToHost.
+    Variable pgm: string.
+    Variable dec: Decoder.Decoder.
+    Variable exec: Decoder.Executer.
+    Variable rf: string.
+    Variable mem: string.
+    Variable toHost: string.
         (* method bindings *)
-    Let d2eFifo := mkFIFO D2E (instancePrefix--"d2eFifo").
-    Let e2wFifo := mkFIFO E2W (instancePrefix--"e2wFifo").
-    Let mem := mkMemory (instancePrefix--"mem").
-    Let rf := mkProcRegs (instancePrefix--"rf").
-    Let sb := mkScoreboard (instancePrefix--"sb").
-    Let decoder := mkPipelinedDecoder (instancePrefix--"decoder") (pgm)%bk (dec)%bk (d2eFifo)%bk.
-    Let executer := mkPipelinedExecuter (instancePrefix--"executer") (d2eFifo)%bk (e2wFifo)%bk (sb)%bk (exec)%bk (rf)%bk (mem)%bk (toHost)%bk.
+    Let d2eFifo_reg : string := instancePrefix--"d2eFifo_reg".
+    Let d2eFifo_valid : string := instancePrefix--"d2eFifo_valid".
+    Let e2wFifo_reg : string := instancePrefix--"e2wFifo_reg".
+    Let e2wFifo_valid : string := instancePrefix--"e2wFifo_valid".
+    Let decoder_pc : string := instancePrefix--"decoder_pc".
+    Let sbFlags : string := instancePrefix--"sbFlags".
+    (* instance methods *)
+    Let mem'doMem : string := mem--"doMem".
+    Let toHost'toHost : string := toHost--"toHost".
     Local Open Scope kami_expr.
 
     Definition mkDecExecSepModule: Mod :=
          (BKMODULE {
-        (BKMod (FIFO'mod d2eFifo :: nil))
-    with (BKMod (FIFO'mod e2wFifo :: nil))
-    with (BKMod (Memory'mod mem :: nil))
-    with (BKMod (ProcRegs'mod rf :: nil))
-    with (BKMod (Scoreboard'mod sb :: nil))
-    with (BKMod (Empty'mod decoder :: nil))
-    with (BKMod (Empty'mod executer :: nil))
+        Register d2eFifo_reg : D2E <- Default
+    with Register d2eFifo_valid : Bool <- (false)%kami_expr
+    with Register e2wFifo_reg : E2W <- Default
+    with Register e2wFifo_valid : Bool <- (false)%kami_expr
+    with Register decoder_pc : Bit PgmSz <-  (* intwidth *) (natToWord PgmSz 0)
+    with Register sbFlags : Array NumRegs Bool <- Default
+    with Rule instancePrefix--"decode" :=
+    (
+        Read d2eFifo_valid_v : Bool <- d2eFifo_valid ;
+        Read decoder_pc_v : Bit PgmSz <- decoder_pc ;
+        Read d2eFifo_reg_v : D2E <- d2eFifo_reg ;
+               LET d2e : D2E (* non-call varbinding *) <- #d2eFifo_reg_v ;
+
+        Assert((!#d2eFifo_valid_v)) ;
+       Read instrs : Array NumInstrs (Bit InstrSz) <- pgm ;
+       LET inst : Bit InstrSz <- #instrs @[ #decoder_pc_v ] ;
+       LET op : OpK (* varbinding *) <-  getOp dec _ inst ;
+       LET arithOp : OpArithK (* varbinding *) <-  getArithOp dec _ inst ;
+       LET src1 : Bit RegFileSz (* varbinding *) <-  getSrc1 dec _ inst ;
+       LET src2 : Bit RegFileSz (* varbinding *) <-  getSrc2 dec _ inst ;
+       LET dst : Bit RegFileSz (* varbinding *) <-  getDst dec _ inst ;
+       LET addr : Bit AddrSz (* varbinding *) <- getAddr dec _ inst ;
+               LET decoded : D2E (* non-call varbinding *) <- STRUCT { "addr" ::= (#addr) ; "arithOp" ::= (#arithOp) ; "dst" ::= (#dst) ; "op" ::= (#op) ; "pc" ::= (#decoder_pc_v) ; "src1" ::= (#src1) ; "src2" ::= (#src2)  }%kami_expr ;
+               Write d2eFifo_reg : D2E <- #decoded ;
+               Write d2eFifo_valid : Bool <- ($$true)%kami_expr ;
+               Write decoder_pc : Bit PgmSz <- (#decoder_pc_v + $$ (* intwidth *) (natToWord PgmSz 1)) ;
+        Retv ) (* rule decode *)
+    with Rule instancePrefix--"executeArith" :=
+    (
+        Read d2eFifo_valid_v : Bool <- d2eFifo_valid ;
+        Read e2wFifo_valid_v : Bool <- e2wFifo_valid ;
+        Read sbFlags_v : Array NumRegs Bool <- sbFlags ;
+        Read d2eFifo_reg_v : D2E <- d2eFifo_reg ;
+               LET d2e : D2E (* non-call varbinding *) <- #d2eFifo_reg_v ;
+
+        Assert(((((((#d2e @% "op") == $$ (* isConstT *)opArith) && (!(#sbFlags_v @[ (#d2e @% "src1") ]))) && (!(#sbFlags_v @[ (#d2e @% "src2") ]))) && #d2eFifo_valid_v) && (!#e2wFifo_valid_v))) ;
+               Write d2eFifo_valid : Bool <- ($$false)%kami_expr ;
+               LET src1 : Bit RegFileSz (* non-call varbinding *) <- (#d2e @% "src1") ;
+               LET src2 : Bit RegFileSz (* non-call varbinding *) <- (#d2e @% "src2") ;
+               LET dst : Bit RegFileSz (* non-call varbinding *) <- (#d2e @% "dst") ;
+               LET arithOp : OpArithK (* non-call varbinding *) <- (#d2e @% "arithOp") ;
+       Read regsval : Array NumRegs (Bit DataSz) <- rf ;
+       LET val1 : Bit DataSz (* varbinding *) <-  #regsval @[ #src1 ] ;
+       LET val2 : Bit DataSz (* varbinding *) <-  #regsval @[ #src2 ] ;
+
+       LET execVal : Bit DataSz <- (execArith exec _ arithOp val1 val2) ;
+               LET flags : Array NumRegs Bool (* non-call varbinding *) <- #sbFlags_v ;
+               LET flags : Array NumRegs Bool <- #flags @[#dst <- $$true ] ;
+               Write sbFlags : Array NumRegs Bool <- #flags ;
+               LET e2w : E2W (* non-call varbinding *) <- STRUCT { "idx" ::= (#dst) ; "val" ::= (#execVal)  }%kami_expr ;
+               Write e2wFifo_reg : E2W <- #e2w ;
+               Write e2wFifo_valid : Bool <- ($$true)%kami_expr ;
+        Retv ) (* rule executeArith *)
+    with Rule instancePrefix--"executeLoad" :=
+    (
+        Read d2eFifo_valid_v : Bool <- d2eFifo_valid ;
+        Read e2wFifo_valid_v : Bool <- e2wFifo_valid ;
+        Read sbFlags_v : Array NumRegs Bool <- sbFlags ;
+        Read d2eFifo_reg_v : D2E <- d2eFifo_reg ;
+               LET d2e : D2E (* non-call varbinding *) <- #d2eFifo_reg_v ;
+
+        Assert(((((((#d2e @% "op") == $$ (* isConstT *)opLd) && (!(#sbFlags_v @[ (#d2e @% "src1") ]))) && (!(#sbFlags_v @[ (#d2e @% "dst") ]))) && #d2eFifo_valid_v) && (!#e2wFifo_valid_v))) ;
+               Write d2eFifo_valid : Bool <- ($$false)%kami_expr ;
+               LET src1 : Bit RegFileSz (* non-call varbinding *) <- (#d2e @% "src1") ;
+               LET dst : Bit RegFileSz (* non-call varbinding *) <- (#d2e @% "dst") ;
+               LET addr : Bit AddrSz (* non-call varbinding *) <- (#d2e @% "addr") ;
+       Read regsval : Array NumRegs (Bit DataSz) <- rf ;
+       LET val1 : Bit DataSz (* varbinding *) <-  #regsval @[ #src1 ] ;
+
+               LET memrq : MemRq (* non-call varbinding *) <- STRUCT { "addr" ::= (#addr) ; "data" ::= ($$ (* intwidth *) (natToWord 32 0)) ; "isLoad" ::= ($$ (* intwidth *) (natToWord 1 1))  }%kami_expr ;
+               BKCall ldVal : Bit DataSz (* actionBinding *) <- mem'doMem ((#memrq) : MemRq) ;
+               LET flags : Array NumRegs Bool (* non-call varbinding *) <- #sbFlags_v ;
+               LET flags : Array NumRegs Bool <- #flags @[ #dst <- $$true ] ;
+               Write sbFlags : Array NumRegs Bool <- #flags ;
+               LET e2w : E2W (* non-call varbinding *) <- STRUCT { "idx" ::= (#dst) ; "val" ::= (#ldVal)  }%kami_expr ;
+               Write e2wFifo_reg : E2W <- #e2w ;
+               Write e2wFifo_valid : Bool <- ($$true)%kami_expr ;
+        Retv ) (* rule executeLoad *)
+    with Rule instancePrefix--"executeStore" :=
+    (
+        Read d2eFifo_valid_v : Bool <- d2eFifo_valid ;
+        Read sbFlags_v : Array NumRegs Bool <- sbFlags ;
+        Read d2eFifo_reg_v : D2E <- d2eFifo_reg ;
+               LET d2e : D2E (* non-call varbinding *) <- #d2eFifo_reg_v ;
+
+        Assert(((((#d2e @% "op") == $$ (* isConstT *)opSt) && (!(#sbFlags_v @[ (#d2e @% "src1") ]))) && #d2eFifo_valid_v)) ;
+               Write d2eFifo_valid : Bool <- ($$false)%kami_expr ;
+               LET src1 : Bit RegFileSz (* non-call varbinding *) <- (#d2e @% "src1") ;
+               LET addr : Bit AddrSz (* non-call varbinding *) <- (#d2e @% "addr") ;
+       Read regsval : Array NumRegs (Bit DataSz) <- rf ;
+       LET val1 : Bit DataSz (* varbinding *) <-  #regsval @[ #src1 ] ;
+
+               LET memrq : MemRq (* non-call varbinding *) <- STRUCT { "addr" ::= (#addr) ; "data" ::= (#val1) ; "isLoad" ::= ($$ (* intwidth *) (natToWord 1 0))  }%kami_expr ;
+               BKCall unused : Bit DataSz (* actionBinding *) <- mem'doMem ((#memrq) : MemRq) ;
+        Retv ) (* rule executeStore *)
+    with Rule instancePrefix--"executeToHost" :=
+    (
+        Read d2eFifo_valid_v : Bool <- d2eFifo_valid ;
+        Read sbFlags_v : Array NumRegs Bool <- sbFlags ;
+        Read d2eFifo_reg_v : D2E <- d2eFifo_reg ;
+               LET d2e : D2E (* non-call varbinding *) <- #d2eFifo_reg_v ;
+
+        Assert(((((#d2e @% "op") == $$ (* isConstT *)opTh) && (!(#sbFlags_v @[ (#d2e @% "src1") ]))) && #d2eFifo_valid_v)) ;
+               Write d2eFifo_valid : Bool <- ($$false)%kami_expr ;
+               LET src1 : Bit RegFileSz (* non-call varbinding *) <- (#d2e @% "src1") ;
+               LET addr : Bit AddrSz (* non-call varbinding *) <- (#d2e @% "addr") ;
+       Read regsval : Array NumRegs (Bit DataSz) <- rf ;
+       LET val1 : Bit DataSz (* varbinding *) <-  #regsval @[ #src1 ] ;
+
+               BKCall unused : Void (* actionBinding *) <- toHost'toHost ((#val1) : Bit DataSz) ;
+        Retv ) (* rule executeToHost *)
     }). (* mkDecExecSep *)
 
-(* Module mkDecExecSep type RegFile#(Bit#(PgmSz), Bit#(InstrSz)) -> Decoder -> Executer -> ToHost -> Module#(Empty) return type Decoder *)
-    Definition mkDecExecSep := Build_Empty mkDecExecSepModule%kami.
+    Hint Unfold mkDecExecSepModule : ModuleDefs.
+(* Module mkDecExecSep type RegFile#(Bit#(PgmSz), Bit#(InstrSz)) -> Decoder -> Executer -> ProcRegs -> Memory -> ToHost -> Module#(Empty) return type Decoder *)
+    Definition mkDecExecSep := Build_Empty mkDecExecSepModule.
+    Hint Unfold mkDecExecSep : ModuleDefs.
+    Hint Unfold mkDecExecSepModule : ModuleDefs.
+
     End Section'mkDecExecSep.
 End module'mkDecExecSep.
 
