example/out/ProcMemInterm.v
@@ -22,26 +22,30 @@ Module module'mkProcInterm.
     Variable mem: Memory.
     Variable toHost: ToHost.
         (* method bindings *)
-    Let pc := mkReg (instancePrefix--"pc") ($0)%bk.
-    Let rf := mkProcRegs (instancePrefix--"rf").
-    Let sb := mkScoreboard (instancePrefix--"sb").
-    Let e2wFifo := mkFIFO (instancePrefix--"e2wFifo").
-    Let decexec := mkDecExec (instancePrefix--"decexec") (pgm)%bk (dec)%bk (exec)%bk (sb)%bk (e2wFifo)%bk (rf)%bk (mem)%bk (toHost)%bk.
-    Let writeback := mkPipelinedWriteback (instancePrefix--"writeback") (e2wFifo)%bk (sb)%bk (rf)%bk.
+    Let pc : string := instancePrefix--"pc".
+    Let (* action binding *) rf := mkProcRegs (instancePrefix--"rf").
+    Let (* action binding *) sb := mkScoreboard (instancePrefix--"sb").
+    Let e2wFifo_reg : string := instancePrefix--"e2wFifo_reg".
+    Let e2wFifo_valid : string := instancePrefix--"e2wFifo_valid".
+    Let (* action binding *) decexec := mkDecExec (instancePrefix--"decexec") (pgm)%bk (dec)%bk (exec)%bk (e2wFifo_reg_v)%bk (e2wFifo_valid_v)%bk (rf)%bk (mem)%bk (toHost)%bk.
     Local Open Scope kami_expr.
 
     Definition mkProcIntermModule: Mod :=
          (BKMODULE {
-        (BKMod (Reg'mod pc :: nil))
+        Register pc : Bit PgmSz <- $ (* int *) 0
     with (BKMod (ProcRegs'mod rf :: nil))
     with (BKMod (Scoreboard'mod sb :: nil))
-    with (BKMod (FIFO'mod e2wFifo :: nil))
+    with Register e2wFifo_reg : E2W <- Default
+    with Register e2wFifo_valid : Bool <- ($$false)%kami_expr
     with (BKMod (Empty'mod decexec :: nil))
-    with (BKMod (Empty'mod writeback :: nil))
     }). (* mkProcInterm *)
 
+    Hint Unfold mkProcIntermModule : ModuleDefs.
 (* Module mkProcInterm type RegFile#(Bit#(PgmSz), Bit#(InstrSz)) -> Decoder -> Executer -> Memory -> ToHost -> Module#(Empty) return type Decoder *)
-    Definition mkProcInterm := Build_Empty mkProcIntermModule%kami.
+    Definition mkProcInterm := Build_Empty mkProcIntermModule.
+    Hint Unfold mkProcInterm : ModuleDefs.
+    Hint Unfold mkProcIntermModule : ModuleDefs.
+
     End Section'mkProcInterm.
 End module'mkProcInterm.
 
