example/out/RegFile.v
@@ -6,4 +6,3 @@ Require Import Bsvtokami.
 Require Import FunctionalExtensionality.
 
 Set Implicit Arguments.
-
