example/out/Vector.v
@@ -1,8 +1,6 @@
 Require Import Bool String List Arith.
 Require Import Omega.
-Require Import micromega.Lia.
-Require Import Kami.
-Require Import Lib.Indexer.
+Require Import Kami.All.
 Require Import Bsvtokami.
 
 Require Import FunctionalExtensionality.
@@ -12,8 +10,8 @@ Set Implicit Arguments.
 
 (* * interface Vector#(len, element_type) *)
 Record Vector := {
-    Vector'modules: Modules;
+    Vector'mod: Mod;
 }.
 
-Hint Unfold Vector'modules : ModuleDefs.
+Hint Unfold Vector'mod : ModuleDefs.
 
