example/ProcDecExec.bsv
@@ -7,42 +7,43 @@ import PipelinedProc::*;
 module mkDecExec#(RegFile#(Bit#(PgmSz), Bit#(InstrSz)) pgm,
 		  Decoder dec,
                   Executer exec,
-		  Scoreboard sb,
 		  FIFO#(E2W) e2wFifo,
-		  ProcRegs rf,
+		  Reg#(Vector#(NumRegs, Bit#(DataSz))) rf,
 		  Memory mem,
 		  ToHost toHost)(Empty);
    Reg#(Bit#(PgmSz)) pc <- mkReg(0);
 
+   RegFile#(Bit#(RegFileSz), Bool) sbFlags <- mkRegFileFull();
+
    rule decexecArith if (dec.isOp(pgm.sub(pc), opArith)
-			&& !sb.search1(dec.getSrc1(pgm.sub(pc)))
-			&& !sb.search2(dec.getSrc2(pgm.sub(pc)))
+			&& !sbFlags.sub(dec.getSrc1(pgm.sub(pc)))
+			&& !sbFlags.sub(dec.getSrc2(pgm.sub(pc)))
 			);
       Bit#(InstrSz) inst = pgm.sub(pc);
       Bit#(RegFileSz) src1 = dec.getSrc1(inst);
       Bit#(RegFileSz) src2 = dec.getSrc2(inst);
       Bit#(RegFileSz) dst = dec.getDst(inst);
       OpArithK arithOp = dec.getArithOp(inst);
-      Bit#(DataSz) val1 = rf.read1(src1);
-      Bit#(DataSz) val2 = rf.read2(src2);
+      Bit#(DataSz) val1 = rf[src1];
+      Bit#(DataSz) val2 = rf[src2];
       Bit#(DataSz) execVal = exec.execArith(arithOp, val1, val2);
-      void inserted <- sb.insert(dst);
+      void unused <- sbFlags.upd(dst, True);
       E2W e2w = E2W { idx: dst, val: execVal };
       void enq <- e2wFifo.enq(e2w);
       pc <= pc + 1;
    endrule
 
    rule decexecLd if (dec.isOp(pgm.sub(pc), opLd)
-			&& !sb.search1(dec.getDst(pgm.sub(pc)))
+			&& !sbFlags.sub(dec.getDst(pgm.sub(pc)))
 			);
       Bit#(InstrSz) inst = pgm.sub(pc);
       Bit#(RegFileSz) src1 = dec.getSrc1(inst);
       Bit#(RegFileSz) dst = dec.getDst(inst);
       Bit#(AddrSz) addr = dec.getAddr(inst);
-      Bit#(DataSz) val1 = rf.read1(src1);
+      Bit#(DataSz) val1 = rf[src1];
       MemRq memrq = MemRq { isLoad: 1'b1, addr: addr, data: val1 };
       Bit#(DataSz) ldVal <- mem.doMem(memrq);
-      void inserted <- sb.insert(dst);
+      void unused <- sbFlags.upd(dst, True);
       E2W e2w = E2W { idx: dst, val: ldVal };
       void enq <- e2wFifo.enq(e2w);
       pc <= pc + 1;
@@ -52,18 +53,18 @@ module mkDecExec#(RegFile#(Bit#(PgmSz), Bit#(InstrSz)) pgm,
       Bit#(InstrSz) inst = pgm.sub(pc);
       Bit#(RegFileSz) src1 = dec.getSrc1(inst);
       Bit#(AddrSz) addr = dec.getAddr(inst);
-      Bit#(DataSz) val1 = rf.read1(src1);
+      Bit#(DataSz) val1 = rf[src1];
       MemRq memrq = MemRq { isLoad: 1'b0, addr: addr, data: val1 };
       Bit#(DataSz) unused <- mem.doMem(memrq);
       pc <= pc + 1;
    endrule
 
    rule decexecToHost if (dec.isOp(pgm.sub(pc), opTh)
-			&& !sb.search1(dec.getSrc1(pgm.sub(pc)))
+			&& !sbFlags.sub(dec.getSrc1(pgm.sub(pc)))
 			);
       Bit#(InstrSz) inst = pgm.sub(pc);
       Bit#(RegFileSz) src1 = dec.getSrc1(inst);
-      Bit#(DataSz) val1 = rf.read1(src1);
+      Bit#(DataSz) val1 = rf[src1];
       void unused <- toHost.toHost(val1);
       pc <= pc + 1;
    endrule
@@ -73,18 +74,89 @@ endmodule
 module mkDecExecSep#(RegFile#(Bit#(PgmSz), Bit#(InstrSz)) pgm,
 		     Decoder dec,
 		     Executer exec,
+		     Memory mem,
+                     Reg#(Vector#(NumRegs, Bit#(DataSz))) rf;
 		     ToHost toHost)(Empty);
    FIFO#(D2E) d2eFifo <- mkFIFO();
    FIFO#(E2W) e2wFifo <- mkFIFO();
-   Memory mem <- mkMemory();
-   ProcRegs rf <- mkProcRegs();
-   Scoreboard sb <- mkScoreboard();
-   Empty decoder <- mkPipelinedDecoder(pgm, dec, d2eFifo);
-   Empty executer <- mkPipelinedExecuter(d2eFifo,
-                                         e2wFifo,
-                                         sb,
-                                         exec,
-                                         rf,
-					 mem,
-					 toHost);
+
+   Reg#(Bit#(PgmSz)) decoder_pc <- mkReg(16'h0);
+   RegFile#(Bit#(RegFileSz), Bool) sbFlags <- mkRegFileFull();
+
+   rule decode;
+      Bit#(InstrSz) inst = pgm.sub(decoder_pc);
+      OpK op = dec.getOp(inst);
+      OpArithK arithOp = dec.getArithOp(inst);
+      Bit#(RegFileSz) src1 = dec.getSrc1(inst);
+      Bit#(RegFileSz) src2 = dec.getSrc2(inst);
+      Bit#(RegFileSz) dst = dec.getDst(inst);
+      Bit#(AddrSz) addr = dec.getAddr(inst);
+
+      D2E decoded = D2E {
+         op: op, arithOp: arithOp, src1: src1, src2: src2, dst: dst, addr: addr, pc: decoder_pc
+         };
+      void enq <- d2eFifo.enq(decoded);
+      decoder_pc <= decoder_pc + 16'd1;
+
+   endrule
+
+   D2E d2e = d2eFifo.first();
+   rule executeArith if (d2e.op == opArith
+                         && !sbFlags.sub(d2e.src1)
+                         && !sbFlags.sub(d2e.src2)
+                        );
+      D2E d2e = d2eFifo.first();
+      void deq <- d2eFifo.deq();
+      Bit#(RegFileSz) src1 = d2e.src1;
+      Bit#(RegFileSz) src2 = d2e.src2;
+      Bit#(RegFileSz) dst = d2e.dst;
+      OpArithK arithOp = d2e.arithOp;
+      Bit#(DataSz) val1 = rf[src1];
+      Bit#(DataSz) val2 = rf[src2];
+      Bit#(DataSz) execVal = exec.execArith(arithOp, val1, val2);
+      void unused <- sbFlags.upd(dst, True);
+      E2W e2w = E2W { idx: dst, val: execVal };
+      void enq <- e2wFifo.enq(e2w);
+   endrule
+
+   rule executeLoad if (d2e.op == opLd
+                         && !sbFlags.sub(d2e.src1)
+                         && !sbFlags.sub(d2e.dst)
+                        );
+      D2E d2e = d2eFifo.first();
+      void deq <- d2eFifo.deq();
+      Bit#(RegFileSz) src1 = d2e.src1;
+      Bit#(RegFileSz) dst = d2e.dst;
+      Bit#(AddrSz) addr = d2e.addr;
+      Bit#(DataSz) val1 = rf[src1];
+      MemRq memrq = MemRq { isLoad: 1'b1, addr: addr, data: 32'b0 };
+      Bit#(DataSz) ldVal <- mem.doMem(memrq);
+      void unused <- sbFlags.upd(dst, True);
+      E2W e2w = E2W { idx: dst, val: ldVal };
+      void enq <- e2wFifo.enq(e2w);
+   endrule
+
+   rule executeStore if (d2e.op == opSt
+                         && !sbFlags.sub(d2e.src1)
+                        );
+      D2E d2e = d2eFifo.first();
+      void deq <- d2eFifo.deq();
+      Bit#(RegFileSz) src1 = d2e.src1;
+      Bit#(AddrSz) addr = d2e.addr;
+      Bit#(DataSz) val1 = rf[src1];
+      MemRq memrq = MemRq { isLoad: 1'b0, addr: addr, data: val1 };
+      Bit#(DataSz) unused <- mem.doMem(memrq);
+   endrule
+
+   rule executeToHost if (d2e.op == opTh
+                         && !sbFlags.sub(d2e.src1)
+                        );
+      D2E d2e = d2eFifo.first();
+      void deq <- d2eFifo.deq();
+      Bit#(RegFileSz) src1 = d2e.src1;
+      Bit#(AddrSz) addr = d2e.addr;
+      Bit#(DataSz) val1 = rf[src1];
+      void unused <- toHost.toHost(val1);
+   endrule
+
 endmodule
