example/ProcMemInterm.bsv
@@ -15,6 +15,7 @@ module mkProcInterm#(RegFile#(Bit#(PgmSz), Bit#(InstrSz)) pgm,
    ProcRegs rf <- mkProcRegs();
    Scoreboard sb <- mkScoreboard();
    FIFO#(E2W) e2wFifo <- mkFIFO();
-   Empty decexec <- mkDecExec(pgm, dec, exec, sb, e2wFifo, rf, mem, toHost);
+   Empty decexec <- mkDecExec(pgm, dec, exec, // sb,
+      e2wFifo, rf, mem, toHost);
    Empty writeback <- mkPipelinedWriteback(e2wFifo, sb, rf);
 endmodule
